reverted to explicit typing for bound terms + cat

src/TL.lean
@@ -5,6 +5,7 @@ Author: Billy Price
 -/
 
 import data.finset
+import tactic.tidy
 namespace TT
 
 inductive type : Type
@@ -13,7 +14,7 @@ inductive type : Type
 notation `Ω` := type.Omega
 def Unit := type.Unit
 infix `××`:max := type.Prod
-prefix 𝒫 :max := type.Pow
+notation `𝒫`A :max := type.Pow A
 
 def context := list type
 
@@ -27,9 +28,11 @@ inductive term : Type
 | elem : term → term → term
 | pair : term → term → term
 | var  : ℕ → term
-| comp : term → term
-| all  : term → term
-| ex   : term → term
+| comp : type → term → term
+| all  : type → term → term
+| ex   : type → term → term
+
+open term
 
 -- * * * * * * * * * * * * * * * * * * * * * * * * * * * * * * * * * * * * * * * 
 -- Notation and derived operators 
@@ -57,164 +60,258 @@ infix ` ⇔ `:60 := iff -- input \<=>
 
 infix ∈ := term.elem
 infix ∉ := λ a α, not (term.elem a α)
-notation `⟦` φ `⟧` := term.comp φ
+notation `⟦ ` A ` | ` φ ` ⟧` := term.comp A φ
 
 notation `⟪` a `,` b `⟫` := term.pair a b 
 
-prefix `∀'`:1 := term.all 
-prefix `∃'`:2 := term.ex
+notation `∀'` := term.all
+notation `∃'` := term.ex
 
-def eq (a₁ a₂ : term) : term := ∀' (a₁ ∈ 𝟘) ⇔ (a₂ ∈ 𝟘)
-infix `≃` :50 := eq
 
-def singleton (a : term) := ⟦a ≃ (𝟘)⟧
+section substitution
 
-def ex_unique (φ : term) : term :=
-  ∃' ⟦φ⟧ ≃ singleton (𝟛)
+  @[simp]
+  def lift_d (d : ℕ) : ℕ → term → term
+  | k ⁎          := ⁎
+  | k ⊤          := ⊤
+  | k ⊥          := ⊥
+  | k (p ⋀ q)    := (lift_d k p) ⋀ (lift_d k q)
+  | k (p ⋁ q)    := (lift_d k p) ⋁ (lift_d k q)
+  | k (p ⟹ q)   := (lift_d k p) ⟹ (lift_d k q)
+  | k (a ∈ α)    := (lift_d k a) ∈ (lift_d k α)
+  | k ⟪a,b⟫      := ⟪lift_d k a, lift_d k b⟫
+  | k (var m)    := if m≥k then var (m+d) else var m
+  | k ⟦A | φ⟧     :=   ⟦A | lift_d (k+1) φ⟧
+  | k (∀' A φ)   := ∀' A $ lift_d (k+1) φ
+  | k (∃' A φ)   := ∃' A $ lift_d (k+1) φ
+
+  @[simp]
+  def lift := lift_d 1 0
+
+  @[simp]
+  def subst : ℕ → term → term → term
+  | n x ⁎          := ⁎
+  | n x ⊤          := ⊤
+  | n x ⊥          := ⊥
+  | n x (p ⋀ q)    := (subst n x p) ⋀ (subst n x q)
+  | n x (p ⋁ q)    := (subst n x p) ⋁ (subst n x q)
+  | n x (p ⟹ q)  := (subst n x p) ⟹ (subst n x q)
+  | n x (a ∈ α)    := (subst n x a) ∈ (subst n x α)
+  | n x ⟪a,c⟫      := ⟪subst n x a, subst n x c⟫
+  | n x (var m)    := if n=m then x else var m
+  | n x ⟦ A | φ ⟧   :=    ⟦A | subst (n+1) (lift x) φ⟧
+  | n x (∀' A φ)     := ∀' A (subst (n+1) (lift x) φ)
+  | n x (∃' A φ)     := ∃' A (subst (n+1) (lift x) φ)
+
+  notation  `⁅` φ ` // `  b `⁆` := subst 0 b φ
+
+  #reduce ⁅𝟘 // ⊤ ⋀ ⊥⁆
+  #reduce ⁅ 𝟙 // ⊤ ⋀ ⊥⁆
+
+end substitution
+
+def eq (A:type) (a₁ a₂ : term) : term := ∀' (𝒫 A) $ ((lift a₁) ∈ 𝟘) ⇔ ((lift a₂) ∈ 𝟘)
+notation a ` ≃[`:max A `] `:0 b := eq A a b
+
+#check eq Unit 𝟘 𝟘
+
+def singleton (A : type) (a : term) := ⟦A | (lift a) ≃[A] 𝟘⟧
+
+def ex_unique (A : type) (φ : term) : term :=
+  ∃' A (⟦A | φ⟧ ≃[𝒫 A] (singleton A 𝟘))
 prefix `∃!'`:2 := ex_unique
 
-def subseteq (α : term) (β : term) : term :=
-  ∀' (𝟘 ∈ α) ⟹ (𝟘 ∈ β)
-infix ⊆ := subseteq
+def subseteq (A : type) (α : term) (β : term) : term :=
+  ∀' A (𝟘 ∈ (lift α)) ⟹ (𝟘 ∈ (lift β))
+notation a ` ⊆[`:max A `] `:0 b := subseteq A a b
 
-def set_prod {A B : type} (α β : term) : term :=
-  ⟦∃' ∃' (𝟙 ∈ α) ⋀ (𝟘 ∈ β) ⋀ (𝟛 ≃ ⟪𝟚,𝟙⟫)⟧
+def term_prod (A B : type) (α β : term) : term :=
+  ⟦ A ×× B | ∃' A (∃' B ((𝟙 ∈ α) ⋀ (𝟘 ∈ β) ⋀ (𝟚 ≃[A××B] ⟪𝟙,𝟘⟫)))⟧
+-- notation α ` ××[`:max A,B `] `:0 β := term_prod A B α β
+
+
+@[simp]
+lemma subst.subseteq {x n α β A}: subst n x (α ⊆[A] β) = (subst n x α) ⊆[A] (subst n x β) :=
+  sorry
 
 -- * * * * * * * * * * * * * * * * * * * * * * * * * * * * * * * * * * * * * * *
 open term
 
+@[user_attribute]
+meta def WF_rules : user_attribute :=
+{ name := `TT.WF_rules,
+  descr := "lemmas usable to prove Well Formedness" }
 
-section wellformedness
+inductive WF : context → type → term → Prop
+| star {Γ}         : WF Γ Unit ⁎
+| top  {Γ}         : WF Γ Ω ⊤
+| bot  {Γ}         : WF Γ Ω ⊥
+| and  {Γ p q}     : WF Γ Ω p → WF Γ Ω q → WF Γ Ω (p ⋀ q)
+| or   {Γ p q}     : WF Γ Ω p → WF Γ Ω q → WF Γ Ω (p ⋁ q)
+| imp  {Γ p q}     : WF Γ Ω p → WF Γ Ω q → WF Γ Ω (p ⟹ q)
+| elem {Γ A a α}   : WF Γ A a → WF Γ (𝒫 A) α → WF Γ Ω (a ∈ α)
+| pair {Γ A B a b} : WF Γ A a → WF Γ B b → WF Γ (A ×× B) ⟪a,b⟫
+| var  {Γ A n}     : list.nth Γ n = some A → WF Γ A (var n)
+| comp {Γ A φ}     : WF (A::Γ) Ω φ → WF Γ (𝒫 A) ⟦A | φ⟧
+| all  {Γ A φ}     : WF (A::Γ) Ω φ → WF Γ Ω (∀' A φ)
+| ex   {Γ A φ}     : WF (A::Γ) Ω φ → WF Γ Ω (∃' A φ)
 
-  inductive WF : context → type → term → Prop
-  | star {Γ}         : WF Γ Unit ⁎
-  | top  {Γ}         : WF Γ Ω ⊤
-  | bot  {Γ}         : WF Γ Ω ⊥
-  | and  {Γ p q}     : WF Γ Ω p → WF Γ Ω q → WF Γ Ω (p ⋀ q)
-  | or   {Γ p q}     : WF Γ Ω p → WF Γ Ω q → WF Γ Ω (p ⋁ q)
-  | imp  {Γ p q}     : WF Γ Ω p → WF Γ Ω q → WF Γ Ω (p ⟹ q)
-  | elem {Γ A a α}   : WF Γ A a → WF Γ (𝒫 A) α → WF Γ Ω (a ∈ α)
-  | pair {Γ A B a b} : WF Γ A a → WF Γ B b → WF Γ (A ×× B) ⟪a,b⟫
-  | var  {Γ A n}     : list.nth Γ n = some A → WF Γ A (var n)
-  | comp {Γ A φ}     : WF (A::Γ) Ω φ → WF Γ (𝒫 A) ⟦φ⟧
-  | all  {Γ A φ}     : WF (A::Γ) Ω φ → WF Γ Ω (∀' φ)
-  | ex   {Γ A φ}     : WF (A::Γ) Ω φ → WF Γ Ω (∃' φ)
+attribute [TT.WF_rules] WF.star WF.top WF.bot WF.and WF.or WF.imp WF.elem WF.pair WF.var WF.comp WF.all WF.ex
+
+section
+
+variables {Γ Δ : context}
+variables {p q r φ a b α : term}
+variables {A B Ω' : type}
+-- Ω' is just a fake/variable version of Ω so we don't need to bother proving
+-- that it must be Ω itself.'
+
+meta def WF_prover : tactic unit := do `[intro h, cases h, assumption]
+
+lemma WF.and_left   : WF Γ Ω' (p ⋀ q) → WF Γ Ω' p := by WF_prover
+lemma WF.and_right  : WF Γ Ω' (p ⋀ q) → WF Γ Ω' q := by WF_prover
+lemma WF.or_left    : WF Γ Ω' (p ⋁ q) → WF Γ Ω' p := by WF_prover
+lemma WF.or_right   : WF Γ Ω' (p ⋁ q) → WF Γ Ω' q := by WF_prover
+lemma WF.imp_left   : WF Γ Ω' (p ⟹ q) → WF Γ Ω' p := by WF_prover
+lemma WF.imp_right  : WF Γ Ω' (p ⟹ q) → WF Γ Ω' q := by WF_prover
+lemma WF.pair_left  : WF Γ (A ×× B) ⟪a,b⟫ → WF Γ A a := by WF_prover
+lemma WF.pair_right : WF Γ (A ×× B) ⟪a,b⟫ → WF Γ B b := by WF_prover
+lemma WF.comp_elim  : WF Γ (𝒫 A) ⟦A | φ⟧ → WF (A::Γ) Ω φ := by WF_prover
+lemma WF.all_elim   : WF Γ Ω' (∀' A φ) → WF (A::Γ) Ω' φ := by WF_prover
+lemma WF.ex_elim    : WF Γ Ω' (∀' A φ) → WF (A::Γ) Ω' φ := by WF_prover
+@[TT.WF_rules] lemma WF.iff_intro : WF Γ Ω p → WF Γ Ω q → WF Γ Ω (p ⇔ q) :=
+begin
+  intros,
+  apply_rules WF_rules,
+end
+lemma iff_elim : WF Γ Ω' (p ⇔ q) → WF Γ Ω' p ∧ WF Γ Ω' q :=
+  by {intro h, refine and.intro _ _;{cases h, cases h_a, assumption}}
+
+local notation l₁ ++ l₂ := list.append l₁ l₂
+open list
 
 
-  variable {Γ : context}
-  variables p q r φ a b α : term
-  variables {A B Ω' : type}
-  -- Ω' is just a fake/variable version of Ω so we don't need to bother proving
-  -- that it must be Ω itself.
+lemma WF.lift_d (K Δ Γ : context) (A : type) (a : term) : WF (K ++ Γ) A a → WF (K ++ Δ ++ Γ) A (lift_d (length Δ) (length K) a) :=
+begin
+  intro wfa,
+  generalize_hyp e : K ++ Γ = Γ' at wfa,
+  induction wfa generalizing K,
+  case WF.all  : Γ' A' ψ wfψ ih {subst e, constructor, refine ih (A' :: K) _, refl},
+  case WF.ex   : Γ' A' ψ wfψ ih {subst e, constructor, refine ih (A' :: K) _, refl},
+  case WF.comp : Γ' A' ψ wfψ ih {subst e, constructor, refine ih (A' :: K) _, refl},
+  case WF.var  : Γ' A' n h₁ 
+  {
+    subst e,simp,
+    split_ifs with h₂,
+      apply WF.var,
+      rw ←h₁,
+      rw nth_le_nth,
+      rw nth_le_nth,
+    repeat {sorry}
+  },
+  repeat {sorry},
+end
 
-  local notation `ez` := by {intro h, cases h, assumption}
-  lemma WF.and_left   : WF Γ Ω' (p ⋀ q) → WF Γ Ω' p               := ez
-  lemma WF.and_right  : WF Γ Ω' (p ⋀ q) → WF Γ Ω' q               := ez
-  lemma WF.or_left    : WF Γ Ω' (p ⋁ q) → WF Γ Ω' p               := ez
-  lemma WF.or_right   : WF Γ Ω' (p ⋁ q) → WF Γ Ω' q               := ez
-  lemma WF.imp_left   : WF Γ Ω' (p ⟹ q) → WF Γ Ω' p             := ez
-  lemma WF.imp_right  : WF Γ Ω' (p ⟹ q) → WF Γ Ω' q             := ez
-  lemma WF.pair_left  : WF Γ (A ×× B) ⟪a,b⟫ → WF Γ A a            := ez
-  lemma WF.pair_right : WF Γ (A ×× B) ⟪a,b⟫ → WF Γ B b            := ez
-  lemma WF.comp_elim  : WF Γ (𝒫 A) (⟦φ⟧) → WF (A::Γ) Ω φ          := ez
-  lemma WF.all_elim   : WF Γ Ω' (∀' φ) → ∃ A:type, WF (A::Γ) Ω' φ :=
-    by {intro h, cases h, constructor, assumption}
-  lemma WF.ex_elim    : WF Γ Ω' (∀' φ) → ∃ A:type, WF (A::Γ) Ω' φ :=
-    by {intro h, cases h, constructor, assumption}
-  lemma WF.iff_intro : WF Γ Ω p → WF Γ Ω q → WF Γ Ω (p ⇔ q) :=
-    by {intros h₁ h₂, apply WF.and, all_goals {apply WF.imp, assumption, assumption}}
-  lemma WF.iff_elim : WF Γ Ω' (p ⇔ q) → WF Γ Ω' p ∧ WF Γ Ω' q :=
-    by {intro h, apply and.intro, all_goals {cases h, cases h_a, assumption}}
-  lemma WF.eq_intro {Γ} {a₁ a₂} (A : type) : WF ((𝒫 A) :: Γ) A a₁ → WF ((𝒫 A) :: Γ) A a₂ → WF Γ Ω (a₁ ≃ a₂) :=
-    by {intros h₁ h₂, apply WF.all, apply WF.iff_intro, all_goals {apply WF.elem, assumption, apply WF.var, simp}}
+lemma WF.lift {Γ A a B} : WF Γ A a → WF (B :: Γ) A (lift a) :=
+  by {intros, apply WF.lift_d [] [B] Γ, assumption}
 
-end wellformedness
+@[TT.WF_rules]
+lemma WF.eq_intro {Γ} {a₁ a₂} (A : type) : WF Γ A a₁ → WF Γ A a₂ → WF Γ Ω (a₁ ≃[A] a₂) :=
+begin
+  intros,
+  apply WF.all,
+  apply WF.iff_intro;{apply WF.elem, apply WF.lift, assumption, apply WF.var; refl}
+end
 
-section substitution
+lemma WF.lift_closed {a A} : WF [] A a → lift a = a :=
+begin
+  suffices : ∀ G A a, WF G A a → lift_d 1 (list.length G) a = a,
+  { exact this _ _ _ },
+  introv wf,
+  induction wf; simp * at *,
+  exact if_neg (not_le_of_gt (list.nth_eq_some.1 wf_a).fst)
+end
 
-  def lift (d : ℕ) : ℕ → term → term
-  | k ⁎          := ⁎
-  | k ⊤          := ⊤
-  | k ⊥          := ⊥
-  | k (p ⋀ q)    := (lift k p) ⋀ (lift k q)
-  | k (p ⋁ q)    := (lift k p) ⋁ (lift k q)
-  | k (p ⟹ q)   := (lift k p) ⟹ (lift k q)
-  | k (a ∈ α)    := (lift k a) ∈ (lift k α)
-  | k ⟪a,b⟫      := ⟪lift k a, lift k b⟫
-  | k (var m)    := if m≥k then var (m+d) else var m
-  | k ⟦φ⟧         :=    ⟦lift (k+1) φ⟧
-  | k (∀' φ)     := ∀' lift (k+1) φ
-  | k (∃' φ)     := ∃' lift (k+1) φ
+lemma lift_zero_does_nothing {k} {a : term} : lift_d 0 k a = a :=
+  by induction a generalizing k;simp *
 
-  def subst_nth : ℕ → term → term → term
-  | n x ⁎          := ⁎
-  | n x ⊤          := ⊤
-  | n x ⊥          := ⊥
-  | n x (p ⋀ q)    := (subst_nth n x p) ⋀ (subst_nth n x q)
-  | n x (p ⋁ q)    := (subst_nth n x p) ⋁ (subst_nth n x q)
-  | n x (p ⟹ q)  := (subst_nth n x p) ⟹ (subst_nth n x q)
-  | n x (a ∈ α)    := (subst_nth n x a) ∈ (subst_nth n x α)
-  | n x ⟪a,c⟫      := ⟪subst_nth n x a, subst_nth n x c⟫
-  | n x (var m)    := if n=m then x else var m
-  | n x ⟦φ⟧         :=    ⟦subst_nth (n+1) (lift 1 0 x) φ⟧
-  | n x (∀' φ)     := ∀' (subst_nth (n+1) (lift 1 0 x) φ)
-  | n x (∃' φ)     := ∃' (subst_nth (n+1) (lift 1 0 x) φ)
+lemma WF.list_d_closed {a A d} : WF [] A a → lift_d d 0 a = a :=
+begin
+  intro wf,
+  induction d,
+  case nat.zero : {induction a; apply lift_zero_does_nothing,},
+  sorry
+end
 
-  def subst := subst_nth 0
+lemma WF.closed_with_context {Γ a A} : WF [] A a → WF Γ A a :=
+begin
+  intro wf,
+  induction Γ,
+  assumption,
+  sorry
+end
 
-  notation  φ `⁅` b `⁆` := subst b φ
-
-  #reduce 𝟘⁅⊤ ⋀ ⊥⁆
-  #reduce 𝟙⁅⊤ ⋀ ⊥⁆
-
-end substitution
+end
 
 section proofs
 
-  inductive proof : context → term → term → Prop
-  | axm        {Γ φ}         : WF Γ Ω φ → proof Γ φ φ
-  | vac        {Γ φ}         : WF Γ Ω φ → proof Γ φ ⊤
-  | abs        {Γ φ}         : WF Γ Ω φ → proof Γ ⊥ φ
-  | and_intro  {Γ p q r}     : proof Γ p q → proof Γ p r → proof Γ p (q ⋀ r)  
-  | and_left   {Γ} (p q r)   : proof Γ p (q ⋀ r) → proof Γ p q
-  | and_right  {Γ} (p q r)   : proof Γ p (q ⋀ r) → proof Γ p r
-  | or_intro   {Γ p q r}     : proof Γ p r → proof Γ q r → proof Γ (p ⋁ q) r  
-  | or_left    {Γ} (p q r)   : proof Γ (p ⋁ q) r → proof Γ p r
-  | or_right   {Γ} (p q r)   : proof Γ (p ⋁ q) r → proof Γ q r
-  | imp_to_and {Γ p q r}     : proof Γ p (q ⟹ r) → proof Γ (p ⋀ q) r
-  | and_to_imp {Γ p q r}     : proof Γ (p ⋀ q) r → proof Γ p (q ⟹ r)
-  | weakening  {Γ φ ψ B}     : proof Γ φ ψ → proof (list.concat Γ B) φ ψ
-  | cut        {Γ} (φ c ψ)   : proof Γ φ c → proof Γ c ψ → proof Γ φ ψ
-  | all_elim   {Γ p φ B}     : proof Γ p (∀' φ) → proof (B::Γ) p φ
-  | all_intro  {Γ p φ} (B)   : proof (B::Γ) p φ → proof Γ p (∀' φ)
-  | ex_elim    {Γ p φ B}     : proof Γ p (∃' φ) → proof (B::Γ) p φ
-  | ex_intro   {Γ p φ B}     : proof (B::Γ) p φ → proof Γ p (∃' φ)
-  | ext                      : proof [] ⊤ $ ∀' ∀' (∀' (𝟘 ∈ 𝟚) ⇔ (𝟘 ∈ 𝟙)) ⟹ (𝟙 ≃ 𝟘)
-  | prop_ext                 : proof [] ⊤ ∀' ∀' (𝟙 ⇔ 𝟘) ⟹ (𝟚 ≃ 𝟙)
-  | star_unique              : proof [] ⊤ ∀' (𝟙 ≃ ⁎)
-  | pair_exists_rep          : proof [] ⊤ ∀' ∃' ∃' 𝟚 ≃ ⟪𝟙,𝟘⟫
-  | pair_distinct_rep        : proof [] ⊤ ∀' ∀' ∀' ∀' (⟪𝟜,𝟚⟫ ≃ ⟪𝟛,𝟙⟫) ⟹ (𝟜 ≃ 𝟛 ⋀ 𝟚 ≃ 𝟙)
-  | apply      {Γ B} (φ ψ b) : WF Γ B b → proof (B::Γ) φ ψ → proof Γ (φ⁅b⁆) (ψ⁅b⁆)
-  | comp       {Γ φ A}       : WF (A::A::Γ) Ω φ → proof Γ ⊤ (∀' (𝟘 ∈ ⟦φ⟧) ⇔ (φ⁅𝟙⁆))
+inductive proof : context → term → term → Prop
+| axm        {Γ} {φ}       : WF Γ Ω φ → proof Γ φ φ
+| vac        {Γ} {φ}       : WF Γ Ω φ → proof Γ φ ⊤
+| abs        {Γ} {φ}       : WF Γ Ω φ → proof Γ ⊥ φ
+| and_intro  {Γ} {p q r}   : proof Γ p q → proof Γ p r → proof Γ p (q ⋀ r)
+| and_left   {Γ} (p q r)   : proof Γ p (q ⋀ r) → proof Γ p q
+| and_right  {Γ} (p q r)   : proof Γ p (q ⋀ r) → proof Γ p r
+| or_intro   {Γ} {p q r}   : proof Γ p r → proof Γ q r → proof Γ (p ⋁ q) r
+| or_left    {Γ} (p q r)   : proof Γ (p ⋁ q) r → proof Γ p r
+| or_right   {Γ} (p q r)   : proof Γ (p ⋁ q) r → proof Γ q r
+| imp_to_and {Γ} {p q r}   : proof Γ p (q ⟹ r) → proof Γ (p ⋀ q) r
+| and_to_imp {Γ} {p q r}   : proof Γ (p ⋀ q) r → proof Γ p (q ⟹ r)
+| weakening  {Γ} {φ ψ Δ}   : proof Γ φ ψ → proof (list.append Γ Δ) φ ψ
+| cut        {Γ} (φ c ψ)   : proof Γ φ c → proof Γ c ψ → proof Γ φ ψ
+| all_elim   {Γ} {p φ A}   : proof Γ p (∀' A φ) → proof (A::Γ) p φ
+| all_intro  {Γ} {p φ} (A) : proof (A::Γ) p φ → proof Γ p (∀' A φ)
+| ex_elim    {Γ} {p φ A}   : proof Γ p (∃' A φ) → proof (A::Γ) p φ
+| ex_intro   {Γ} {p φ} (A) : proof (A::Γ) p φ → proof Γ p (∃' A φ)
+| extensionality {A}       : proof [] ⊤ $ ∀' (𝒫 A) $ ∀' (𝒫 A) $ (∀' A ((𝟘 ∈ 𝟚) ⇔ (𝟘 ∈ 𝟙))) ⟹ (𝟚 ≃[A] 𝟙)
+| prop_ext                 : proof [] ⊤ $ ∀' Ω $ ∀' Ω (𝟙 ⇔ 𝟘) ⟹ (𝟙 ≃[Ω] 𝟘)
+| star_unique              : proof [] ⊤ $ ∀' Unit (𝟘 ≃[Unit] ⁎)
+| pair_exists_rep {A B}    : proof [] ⊤ $ ∀' (A ×× B) $ ∃' A $ ∃' B $ 𝟚 ≃[A ×× B] ⟪𝟙,𝟘⟫
+| pair_distinct_rep {A B}  : proof [] ⊤ $ ∀' A $ ∀' B $ ∀' A $ ∀' B $ (⟪𝟛,𝟙⟫ ≃[A××B] ⟪𝟚,𝟘⟫) ⟹ (𝟛 ≃[A] 𝟚 ⋀ 𝟙 ≃[B] 𝟘)
+| sub      {Γ} (B) (φ ψ b) : WF Γ B b → proof (B::Γ) φ ψ → proof Γ (⁅φ // b⁆) (⁅ψ // b⁆)
+| comp     {Γ} (A) (φ)     : WF (A::Γ) Ω φ → proof Γ ⊤ (∀' A (𝟘 ∈ ⟦A | φ⟧) ⇔ (⁅φ // 𝟘⁆))
 
-  prefix ⊢ := proof [] ⊤
-  infix ` ⊢ `:50 := proof []
-  notation φ ` ⊢[` Γ:(foldr `,` (h t, list.cons h t) list.nil) `] ` ψ := proof Γ φ ψ
-  notation `⊢[` Γ:(foldr `,` (h t, list.cons h t) list.nil) `] ` ψ := proof Γ ⊤ ψ
+@[user_attribute]
+meta def easy_proofs : user_attribute :=
+{ name := `TT.easy_proofs,
+  descr := "Easy proofs" }
 
-  variables p q : term
+attribute [TT.easy_proofs] proof.axm proof.vac proof.abs proof.and_intro proof.or_intro
 
-  #reduce   ⊢ (p ⋁ ∼p)  -- proof [] ⊤ (or p (imp p ⊥))
-  #reduce q ⊢ (p ⋁ ∼p)  -- proof [] q (or p (imp p ⊥))
-  #reduce   ⊢[Ω,Unit] p -- proof [Ω,Unit] ⊤ p
-  #reduce q ⊢[Ω,Unit] p -- proof [Ω,Unit] q p
 
-  variable {Γ : context}
-  variables φ ψ : term
+prefix `⊨`:1 := proof [] ⊤
+infix ` ⊨ `:50 := proof []
+notation φ ` ⊨[` Γ:(foldr `,` (h t, list.cons h t) list.nil) `] ` ψ := proof Γ φ ψ
+notation `⊨[` Γ:(foldr `,` (h t, list.cons h t) list.nil) `] ` ψ := proof Γ ⊤ ψ
 
-  lemma WF.proof_left  : proof Γ φ ψ → WF Γ Ω φ := sorry
-  lemma WF.proof_right : proof Γ φ ψ → WF Γ Ω ψ := sorry
+section
+  variables p q φ ψ : term
+
+  #reduce   ⊨ (p ⋁ ∼p)  -- proof [] ⊤ (or p (imp p ⊥))
+  #reduce q ⊨ (p ⋁ ∼p)  -- proof [] q (or p (imp p ⊥))
+  #reduce   ⊨[Ω,Unit] p -- proof [Ω,Unit] ⊤ p
+  #reduce q ⊨[Ω,Unit] p -- proof [Ω,Unit] q p
+end 
 
 end proofs
+
+namespace WF
+variable {Γ : context}
+variables p q φ ψ : term
+lemma proof_left  : proof Γ φ ψ → WF Γ Ω φ := sorry
+lemma proof_right : proof Γ φ ψ → WF Γ Ω ψ := sorry
+
+end WF
+
 
 end TT
