src/lemmas.lean
@@ -1,0 +1,83 @@
+import TL
+import tactic.tidy
+
+namespace TT
+
+open proof
+
+
+variables p q r φ ψ : term
+variable {Γ : context}
+
+lemma from_meta_imp (_ : WF Γ Ω φ) (_ : WF Γ Ω ψ) : (proof Γ ⊤ φ → proof Γ ⊤ ψ) → proof Γ φ ψ
+  := sorry
+
+lemma to_meta_imp : proof Γ φ ψ  → proof Γ ⊤ φ → proof Γ ⊤ ψ :=
+  by {intros, apply proof.cut _ φ _, tidy}
+
+lemma from_imp {Γ : context} : proof Γ ⊤ (q ⟹ r) → proof Γ q r :=
+begin
+  intro h₁,
+  apply proof.cut _ (⊤ ⋀ q) _,
+  apply_rules easy_proofs,
+  repeat {
+    apply @WF.imp_left _ q r,
+    exact WF.proof_right _ _ h₁
+  },
+  exact proof.imp_to_and h₁,
+end
+
+lemma to_imp {Γ : context} : proof Γ q r → proof Γ ⊤ (q ⟹ r) :=
+begin
+  intro h₁,
+  apply proof.and_to_imp,
+  apply proof.cut _ q _,
+  apply proof.and_right _ ⊤ _,
+  apply proof.axm,
+  apply WF.and,
+  exact WF.top,
+  apply WF.proof_left q r,
+  tidy
+end
+lemma proof.or_inl (wfq : WF Γ Ω q) (prfp :proof Γ ⊤ p) : proof Γ ⊤ (p ⋁ q) :=
+  by {apply proof.cut _ p _, assumption, apply proof.or_left _ q, apply proof.axm, apply_rules [WF.or, WF.proof_right]}
+lemma proof.or_inr (wfq : WF Γ Ω p) (prfp :proof Γ ⊤ q) : proof Γ ⊤ (p ⋁ q) :=
+  by {apply proof.cut _ q _, assumption, apply proof.or_right _ q, apply proof.axm, apply_rules [WF.or, WF.proof_right]}
+
+lemma proof_of_and_left (_ : WF Γ Ω p) (_ : WF Γ Ω q) : proof Γ (p ⋀ q) p :=
+  by {intros, apply proof.and_left _ p q, apply proof.axm, apply WF.and, tidy}
+lemma proof_of_and_right (_ : WF Γ Ω p) (_ : WF Γ Ω q) : proof Γ (p ⋀ q) q :=
+  by {apply proof.and_right _ p q, apply proof.axm, apply WF.and, tidy}
+
+example (_ : WF Γ Ω p) (_ : WF Γ Ω q) : proof Γ (p ⋀ q) (q ⋀ p) :=
+begin
+  apply proof.and_intro,
+  apply proof_of_and_right,
+  tidy,
+  apply proof_of_and_left,
+  tidy
+end
+
+namespace proof
+open term
+
+lemma eq_sound {A : type} {a₁ a₂ : term} (eq : ⊨ (a₁ ≃[A] a₂)) (φ ψ : term) : proof Γ ⊤ ⁅φ // a₁⁆ → proof Γ ⊤ ⁅φ // a₂⁆ :=
+  by sorry
+
+lemma reverse_extensionality (A : type) : ⊨ (∀' (𝒫 A) $ ∀' (𝒫 A) $ (𝟙 ≃[𝒫 A] 𝟘) ⟹ (∀' A ((𝟘 ∈ 𝟙) ⇔ (𝟘 ∈ 𝟚)))) :=
+begin
+  apply proof.all_intro 𝒫 A,
+  apply proof.all_intro 𝒫 A,
+  apply to_imp,
+  apply from_meta_imp,
+  any_goals {apply_rules WF_rules; refl},
+  intro h,
+  sorry
+end
+
+
+
+end proof
+
+
+end TT
